start formalizing Robust Preservation

CommonST.v
@@ -1,16 +1,55 @@
-Record Components :=
+Require Import TraceModel. 
+Require Import Properties.
+Require Import ClassicalExtras.
+
+Set Implicit Arguments. 
+
+Record level :=
   {
     prg  : Set;
-    ctx  : Set; 
-    plug : prg -> ctx -> prg          
+    ctx  : Set;   
+    plug : prg -> ctx -> prg;
+    sem  : prg -> prop;
+    non_empty_sem : forall P, exists t, sem P t
   }.
 
-Axiom source : Components.
-Axiom target : Components.
-Axiom compile : (prg source) -> (prg target).
+  
+Axiom src : level.
+Axiom tgt : level.
+Axiom compile : (prg src) -> (prg tgt).
+
+Notation "C [ P ]" := (plug _ P C) (at level 50).
+Notation "P ↓" := (compile P) (at level 50). 
 
 
+Definition psem {K : level}
+                (P : prg K)
+                (m : finpref) : Prop := 
+  exists t, prefix m t /\ (sem K) P t.
+
+Definition sat {K : level}
+               (P : prg K)
+               (π : prop) : Prop :=
+  forall t, sem K P t -> π t.
+
+Definition rsat {K : level}
+                (P : prg K)
+                (π : prop) : Prop :=
+  forall C, sat (C [ P ] ) π. 
 
 
+Lemma neg_rsat {K : level} :
+    forall P π, ~ rsat P π <->
+           exists C t, sem K (C [ P ]) t /\ ~ π t.
+Proof.
+   unfold rsat. unfold sat. split.
+  - intros r. rewrite not_forall_ex_not in r.
+    destruct r as [C r]. rewrite not_forall_ex_not in r.
+    destruct r as [t r]. exists C,t. rewrite not_imp in r.
+    assumption.
+  - intros [C [t r]]. rewrite not_forall_ex_not.
+    exists C. rewrite not_forall_ex_not. exists t.
+    rewrite not_imp. assumption.
+Qed.
 
 
