Robustdef.v
@@ -1,0 +1,27 @@
+Require Import TraceModel.
+Require Import Properties.
+Require Import CommonST.
+Require Import ClassicalExtras.
+
+(** *Robust Preservation of π *)
+Definition RP (P : prg src) (π : prop) : Prop :=
+  rsat P π -> rsat (P ↓) π.
+
+Lemma contra_RP (P : prg src) (π : prop) :
+     RP P π <->
+     ((exists C' t', sem tgt (C' [ P ↓ ]) t'  /\ ~ π t') ->
+      (exists C t ,  sem src (C [ P ]) t /\ ~ π t)).
+Proof. 
+   unfold RP. split.
+  - intros H. rewrite contra in H.
+    repeat rewrite neg_rsat in H. assumption.
+  - intros H. rewrite contra.
+    repeat rewrite neg_rsat. assumption.
+Qed.  
+
+(** *RObust Preservation of a class of properties*)
+Definition RclassP (class : prop -> Prop) (P : prg src) (π : prop) : Prop :=
+  forall π, class π -> RP P π.
+
+
+(* Bookmark: line 351, TraceFiniInf.v*)
